\documentclass{article}  %document class

\usepackage{amsmath}     %adding package 

\begin{document}         %begin document command
\begin{equation*}        %equation begin without numbering
\iiint\limits_V f(x,y,z)\,dV = F   %equation
\end{equation*}          %equation end


\begin{equation*}        %equation begin without numbering
\frac{dx}{dy}=x'=\lim_{h \to 0}\frac{f(x+h)-f(x)}{h}  %equation
\end{equation*}          %equation end


\begin{equation*}        %equation begin without numbering
|x|=\begin{cases}
-x, & \text{if $x < 0$}\\   %equation 
x, & \text{if $x \geq 0$} 
\end{cases}
\end{equation*}          %equation end


\begin{equation*}        %equation begin without numbering
F(x)= A_0 + \sum_{n=1}^N\left[ A_n\cos{\left(\frac{2\pi nx}{P}\right)}+B_n\sin{\left(\frac{2\pi nx}{P}\right)}\right]  %equation
\end{equation*}          %equation end


\begin{equation*}        %equation begin without numbering
\sum_n \frac{1}{n^s}=\prod_p \frac{1}{1-\frac{1}{p^s}}
\end{equation*}          %equation end


\begin{equation*}        %equation begin without numbering
m\ddot{x}+c\dot{x}+kx=F_0\sin(2\pi ft)
\end{equation*}          %equation end


\begin{align*}          %for alligning
f(x)\quad &=\quad x^2 + 3x + 5x^2 +8 +6x\\  %line 40,41,42 equation part
&=\quad 6x^2 +9x +8\\
&=\quad x(6x+9)+8
\end{align*}

$$
X=\frac{F_0}{k}\frac{1}{\sqrt{(1-r^2)^2+(2\zeta r)^2}}
$$

\begin{equation*}        %equation begin without numbering
G_{\mu\nu} \equiv R_{\mu\nu}-\frac{1}{2}Rg_{\mu\nu}=\frac{8\pi G}{c^4}T_{\mu\nu}
\end{equation*}\\        %equation end

$$\mathrm{6CO_2+6H_2O \to C_6H_{12}O_6+6O_2}$$   %chemical equation

$$\mathrm{SO_4^{2-}+Ba^{2+} \to BaSO_4 }$$     %chemical equation

\begin{equation*}        %equation begin without numbering
\begin{pmatrix}          %matrix start & below lines contain matrix data
a_{11}&a_{12}&\dots&a_{1n}\\
a_{21}&a_{22}&\dots&a_{2n}\\
\vdots&\vdots&\ddots&\vdots\\
a_{n1}&a_{n2}&\dots&a_{nn}
\end{pmatrix}            %matrix end
\begin{pmatrix}          %matrix begin
v_{1}\\
v_{2}\\
\vdots\\
v_{n}
\end{pmatrix}            %matrix end
=
\begin{pmatrix}          %matrix begin
w_{1}\\
w_{2}\\
\vdots\\
w_{n}
\end{pmatrix}            %matrix end
\end{equation*}

\begin{equation*}
\frac{\partial{\bf{u}}}{\partial{t}}+(\bf{u}\cdot\nabla)\bf{u}-\nu\nabla^2\bf(u)=-\nabla h   %equation part
\end{equation*}          %equation end

\[
\alpha A \beta B \gamma \Gamma \delta \Delta \pi \Pi \omega \Omega %printing symbols
\]
\end{document}            %end of document
